thy/Routing/LinuxRouter.thy
@@ -2,15 +2,13 @@ theory LinuxRouter
 imports Routing "../Simple_Firewall/SimpleFw_Semantics"
 begin
 
-datatype forwarding_decision = ForwardOn string | Drop
-
+term "map port_sel $ routing_table_semantics rt (p_dst p)"
 definition "simple_linux_router rt fw p \<equiv> let
-	rd = routing_table_semantics rt (p_dst p);
-	pt = port_sel (hd rd);
-	fd = simple_fw fw (p_oiface_update (const pt) p) in
-	case fd of 
-		Decision FinalAllow \<Rightarrow> ForwardOn pt |
-		Decision FinalDeny \<Rightarrow> Drop"
-
+	rd = routing_table_semantics rt (p_dst p) in
+	concat (map (\<lambda>pt. case (simple_fw fw (p_oiface_update (const (port_sel pt)) p)) of 
+		Decision FinalAllow \<Rightarrow> [pt] |
+		Decision FinalDeny \<Rightarrow> []
+	) rd)"
+(* Todo: Find something that looks a bit more semantic *)
 
 end
